Theorems.v
@@ -2,73 +2,139 @@ Require Import RAC.Definitions.
 Require Import RAC.Notations.
 Require Import RAC.Utils.
 Require Import RAC.Semantics.
+Require Import RAC.Translation.
+Require Import  Strings.String.
+From Coq Require Import ZArith.ZArith.
 
+
+(* Properties of the semantics *)
 
 Fact eq_env_partial_order :  forall e e' v z, e ⊑ e' ->  z <> UInt /\ z <> UMpz -> (fst e) v = Some z -> (fst e') v = Some z.
 Proof.
-    intros. destruct H with v ; try assumption ; try rewrite H2 in H1 ; try injection H1 as Eq ; subst ; try assumption.
-    - destruct H0 as [uint _]. destruct uint. reflexivity.
-    - destruct H0 as [_ umpz]. destruct umpz. reflexivity.
-    - discriminate.
+    intros. destruct H with v ; try assumption ; try rewrite H2 in H1 ; try injection H1 as Eq ; subst ; now try assumption.
 Qed.
 
-#[global] Hint Constructors c_exp_sem  : core.
-#[global] Hint Constructors c_statement  : core.
-#[global] Hint Constructors c_exp  : core.
-#[global] Hint Constructors c_stmt_sem  : core.
-#[global] Hint Constructors env_partial_order : core.
+
+Fact env_same_ty : forall  (Ω Ω' : Ω) v t, Ω ⊑ Ω' -> t <> None -> type_of_value (fst Ω v) = t -> type_of_value (fst Ω' v) = t.
+Proof.
+    intros. destruct H with v ; subst ;  try now rewrite H2,H3.
+    - destruct H3. 
+        * now rewrite H1,H2.
+        * destruct H1. now rewrite H1,H2.
+    -destruct H3. 
+        * now rewrite H1,H2.
+        * destruct H1. now rewrite H1,H2.
+    - destruct H0. now rewrite H2.
+Qed.
 
 Lemma weakening_of_expression_semantics : 
 forall T env (e : @c_exp T) (x:𝕍),
     env |= e => x <-> (forall env', env ⊑ env' ->  env' |= e => x)
 .
-Proof with auto.
-split.
-- generalize dependent x. induction e.
-    * intros v H env' Inc. inversion H...
+Proof with (eauto using refl_env_partial_order with rac_hint ; try easy).
+    split... generalize dependent x. induction e.
+    * intros v H. inversion H...
     * intros v H env' Inc. inversion H.
-        eapply eq_env_partial_order in Inc ; eauto.
-        split ; congruence.
-    * intros v H env' Inc. inversion H. eauto.
-    * intros. inversion H ; eauto.
-- auto using refl_env_partial_order.
+        eapply eq_env_partial_order in Inc...
+    * intros v H. inversion H...
+    * intros. inversion H...
 Qed.
 
+Open Scope mini_gmp_stmt_scope.
+Open Scope mini_gmp_exp_scope.
 
-Open Scope mini_c_stmt_scope.
+
 Lemma weakening_of_statement_semantics_1 :
     forall Ω₀ M₀ s Ω₁ M₁,
     Ω₀ ⋅ M₀ |= s => Ω₁ ⋅ M₁ <->
-    forall Ω₀' M₀', (Ω₀ , M₀) ⊑ (Ω₀', M₀') ->
-     exists Ω₁' M₁', 
-     (Ω₁ , M₁) ⊑ (Ω₁', M₁') /\  Ω₀' ⋅ M₀' |= s => Ω₁'⋅ M₁'.
-Proof.
-    (* split. 
-    - induction s ; intro H ; inversion H ; subst ; intros.
-        * exists Ω₀'. exists M₀'. split. apply H0. constructor.
-        * exists ((fst Ω₀'){var\z}, (snd Ω₀')). exists M₀'. destruct H0 as [H0 _]. split.
-         ** split. 
-            *** intro x. destruct Ω₀,Ω₀'. apply <- env_partial_order_next. apply (H0 x).
-            *** apply fixme.
-         ** constructor. apply (weakening_of_expression_semantics Ω₀) ; assumption.
+   ( forall Ω₀' M₀', (Ω₀ , M₀) ⊑ (Ω₀', M₀') ->
+     exists Ω₁' M₁', (Ω₁ , M₁) ⊑ (Ω₁', M₁') ->
+     Ω₀' ⋅ M₀' |= s => Ω₁'⋅ M₁').
+Proof with auto with rac_hint.
+     split. 
+    - induction s ; intros ; inversion H0 ; inversion H ; inversion H3.
+        (* skip *)
+        * exists Ω₀',M₀'... 
+
+        (* assign *)
+        * pose ((fst Ω₀'){x\z}, snd Ω₀'). exists p ,M₀'.
+         intros. pose (weakening_of_expression_semantics _gmp_t Ω₀ e z). specialize i. rewrite i in H12. specialize H12 with Ω₀'. clear i.
+         subst. constructor. apply S_Assign... now apply env_same_ty with Ω₀.
+
+         (* pcall *)
+        * subst. exists ((fst Ω₀') {var \ z}, snd Ω₀'), M₁.  
+            intros. constructor. eapply S_FCall ; try eassumption.
+            + intros. admit.
+            + admit.
+
+        (* fcall *)         
+        *  eexists. eexists. intro. constructor. eapply S_PCall ; try eassumption.
+            + admit.
+            + admit.
+
+        (* c seq *)
+        * exists Ω₁, M₁. intro. constructor. apply S_Seq with  env' mem'...  admit. admit.
+
+        (* gmp seq *)
+        * exists Ω₁, M₁. intro. apply GMP_Seq with  env' mem'...  admit. admit.
+
+        (* if true *)
+        * exists Ω₁, M₁. intro. constructor. apply S_IfTrue with z.
+            + admit.
+            + admit. 
+
+        (* if false *)
+        * exists Ω₁, M₁. intro. constructor. apply S_IfFalse.
+            +  pose (weakening_of_expression_semantics _gmp_t Ω₀ cond zero). specialize i. rewrite i in H12. specialize H12 with Ω₀'. clear i.
+                rewrite <- H7 in *. clear H3 H4. apply (H12 H1).
+            + admit.
+        
+        (* while *)
+        * exists Ω₁, M₁. intro. constructor. apply S_While. admit.
+
+        (* assert *)
+        * exists Ω₀', M₀'. intro. constructor. apply S_PAssert with z... apply weakening_of_expression_semantics  with Ω₁... inversion H12...
+
+        (* return *)
+        * exists ((fst Ω₀') {resf \ z}, snd Ω₀'), M₀'. intro. subst. constructor. apply S_Return. admit.
+
+        (* set_i *)
         * admit.
+
+        (* set_z *)
         * admit.
+        
+        (* get_int *)
         * admit.
+
+        (* set_s *)
         * admit.
+
+        (* cmp *)
         * admit.
-        * admit.
-        * admit.
-        * admit.
-    - intros. destruct H with Ω₀ M₀ as [Ω₀' [M₀' [[Inc fixme] H1]]]; subst; clear H. 
-        * constructor ; constructor.
-        * inversion H1 ; subst.
-            ** admit.
-             ** replace  Ω₁ with ((fst Ω₀) {x \ z}, snd Ω₀). replace M₁ with M₀' . apply S_Assign.
-               *** assumption.
-               *** admit.
-               *** admit.
-            ** *)
+
+        (* op *)
+        * admit. 
+    
+    - intros. induction s.
+     * destruct H with Ω₀ M₀. 
+        +  constructor.
+            ++ apply refl_env_partial_order.
+            ++ apply refl_mem_partial_order.
+        + destruct H0. admit.
+
+    * admit.
+    * admit.
+    * admit.
+    * admit.
+    * admit.
+    * admit.
+    * admit.
+    * admit.
+    * admit.
+    * admit.
 Admitted.
+
 
 (* 2 *)
 
@@ -95,6 +161,9 @@ Admitted.
  *)
 
 
+
+(* Proofs of structural properties of the translation *)
+
 (* Theorem absence_of_dangling_pointers :
     forall n (z:=VMpz n) (mem_state:𝓜) (var_env:Ωᵥ), 
         mem_state n <> ⊥ n <-> 
@@ -102,3 +171,252 @@ Admitted.
         ~(exists x', x <> x' -> var_env x <> Some z)
 .
 Admitted. *)
+
+
+
+(* Proofs of the semantics of the macros *)
+
+Fact Mpz_exp_is_var : forall e, exists x, ty e = Mpz -> e = C_Id x Mpz.
+Proof. 
+    intros. destruct e ; try now exists "z".
+    exists var. intro H. unfold Definitions.ty in H. now rewrite H.
+Qed.
+
+
+Lemma semantics_of_the_mpz_assgn_macro :
+    forall e z Ω M v (y:location),
+    Ω ⋅ M |= e ⇝ z ->
+    (fst Ω) v = Some (VMpz y) ->
+    Ω ⋅ M |= (mpz_ASSGN v e) => Ω ⋅ M{y\z}
+.
+Proof.
+    intros. 
+    unfold mpz_ASSGN. destruct (ty e) eqn:TY.
+    - inversion H.
+        * now apply S_set_i.
+        * inversion H1 ; now subst.
+    - unfold ty in TY. destruct e; try easy. subst. inversion H; now inversion H1.
+    - destruct t.
+        * destruct H; destruct H ; try easy ; now destruct H.
+        * destruct e; try easy. inversion H.
+            ** inversion H1. inversion H3. now subst.
+            ** inversion H1 ; try easy. subst. now apply S_set_z with l.
+Qed.
+
+Lemma semantics_of_the_int_assgn_macro :
+    forall e z (ir: Int.inRange z) Ω M v,
+    Ω ⋅ M |= e ⇝ z ->
+    type_of_value ((fst Ω) v) = Some C_Int ->
+    Ω ⋅ M |= (int_ASSGN v e) => ((fst Ω){v\z ⁱⁿᵗ ir}, snd Ω) ⋅ M
+.
+Proof with eauto with rac_hint.
+    intros. 
+    unfold int_ASSGN. destruct (ty e) eqn:TY.
+    - inversion H.
+        * constructor. constructor... subst. inversion H1. subst. 
+            replace ((x) ̇ ⁱⁿᵗ ir) with (VInt x). assumption. admit. (* proof of x ̇ in = x *)
+        * inversion H1 ; now subst.
+    - inversion H ; inversion H1;  inversion H3 ; now subst.
+    - destruct t.
+        * destruct H; destruct H ; try easy ; now destruct H.
+        * destruct e; try easy. inversion H.
+            ** inversion H1.  inversion H3. now subst.
+            ** inversion H1 ; try easy. subst. now apply S_get_int with l.
+Admitted.
+
+Lemma semantics_of_the_Z_assgn_macro_tint :
+    forall z (ir: Int.inRange z) Ω M v,
+    type_of_value ((fst Ω) v) = Some C_Int ->
+    Ω ⋅ M |= (Z_ASSGN C_Int v z) => ((fst Ω){v\z ⁱⁿᵗ ir}, snd Ω) ⋅ M
+.
+Proof.
+    intros. simpl. auto with rac_hint.
+Qed.
+
+Lemma semantics_of_the_Z_assgn_macro_tmpz :
+    forall y (z:ℤ) Ω M v,
+    (fst Ω) v = Some (VMpz y) ->
+    Ω ⋅ M |= (Z_ASSGN Mpz v z) => Ω ⋅ M{y\z}
+.
+Proof with auto using BinaryString.Z_of_of_Z.
+    intros. simpl. apply S_set_s...
+Qed.
+    
+
+Lemma semantics_of_the_cmp_macro :
+    forall (Ω:Ω) (M:𝓜) c e1 e2 v1 v2 z1 z2 l1 l2 a,
+    type_of_value ((fst Ω) c) = Some C_Int ->
+    Ω ⋅ M |= e1 ⇝ z1 ->
+    Ω ⋅ M |= e2 ⇝ z2 ->
+    (
+        (a = VInt sub_one <-> Z.lt z1 z2 ) /\
+        (a = VInt zero <-> z1 = z2) /\
+        (a = VInt one <-> Z.gt z1 z2)
+    ) -> 
+    (fst Ω) v1 = Some (VMpz l1) /\ ( (fst Ω) v2 = Some (VMpz l2)) ->
+    exists M', forall v n, (fst Ω) v = Some (VMpz n) ->
+    ~ ((fst Ω) v1 = (fst Ω) v) /\ ~ ((fst Ω) v2 = (fst Ω) v)  -> M n = M' n -> 
+    Ω ⋅ M |= (CMP c e1 e2 v1 v2) => ((fst Ω){c\a}, snd Ω) ⋅ M'
+    .
+
+Proof with try easy ; auto with rac_hint ; unshelve eauto using Z.ltb_irrefl,Z.gtb_ltb,Z.ltb_lt with rac_hint; auto with rac_hint.
+    intros. destruct H2 as (inf & eq & sup), H3.
+
+    assert (NotInt : 
+        exists M', forall v n, (fst Ω) v = Some (VMpz n) ->
+        ~ ((fst Ω) v1 = (fst Ω) v) /\ ~ ((fst Ω) v2 = (fst Ω) v)  -> M n = M' n -> 
+        Ω ⋅ M |= <{ 
+        (mpz_ASSGN v1 e1); 
+        (mpz_ASSGN v2 e2); 
+        <c = cmp (v1, v2)>
+        }> => ((fst Ω){c\a}, snd Ω) ⋅ M'
+    ). {
+        exists M{l2 \ z2, l1 \ z1}. intros v n VN [Hvneqv1 Hvneqv2] HM.
+        apply GMP_Seq with Ω M{l1\z1}.
+        + apply semantics_of_the_mpz_assgn_macro...
+        + apply GMP_Seq with Ω M{l2\z2,l1\z1}.  
+            ++ apply semantics_of_the_mpz_assgn_macro... admit. 
+            ++ apply S_cmp with (vx:=l1) (vy:=l2) (lx:=z1) (ly:=z2)...
+                * apply GMP_E_Var with z1. assumption. unfold p_map. simpl. 
+                    destruct (Nat.eq_dec l2 l1) as [Neq | Nneq].
+                        ** subst. admit.
+                        ** now destruct (Nat.eq_dec l1 l1).
+                * apply GMP_E_Var with z2. assumption. unfold p_map. simpl.
+                    now destruct (Nat.eq_dec l2 l2) as [Neq | Nneq].
+                *  unfold p_map. simpl. destruct (Nat.eq_dec l2 l1) as [Neq | Nneq].
+                    ** subst. admit.
+                    ** now destruct (Nat.eq_dec l1 l1).
+                * unfold p_map. simpl. destruct (Nat.eq_dec l2 l1) as [Neq | Nneq] ;  now destruct (Nat.eq_dec l2 l2).
+    }
+
+     unfold CMP. destruct (ty e1) eqn:T1, (ty e2) eqn:T2 ;
+
+    (* get rid of impossible void type *)
+    try (unfold ty in T2 ; destruct e2 eqn:X; try easy ; subst ; inversion H1 ; inversion H5; easy) ;
+    try (unfold ty in T1;  destruct e1 eqn:X; try easy; subst; inversion H0; inversion H5; easy);
+    (* when ty e1 & ty e2 != int *)
+    try (exists M{l2\z2,l1\z1} ; intros ; now apply NotInt). clear NotInt.
+
+     
+     (* both ty(e1) = int and ty(e2) = int *)
+     inversion H0; inversion H1; inversion H5; inversion H7 ; try (subst ; easy). clear H8 H9.
+        exists M. intros v l Hv _ _. destruct (Z.lt_trichotomy z1 z2) as [inf' | [ eq' | sup']].
+        
+        (* z1 < z2 *)
+        * assert (cmp := inf'). apply <- inf in inf'. clear eq inf sup. rewrite <- H5, <-H7 in cmp.
+            destruct x,x0. constructor. apply S_IfTrue with one. inversion H4. inversion H6.
+            +  split... subst.  eapply C_E_BinOpTrue... now apply Z.ltb_lt.
+            + constructor... replace a with (⋄ C_Sub 0 1 ⁱⁿᵗ suboneinRange)...
+
+        (* z1 = z2 *)
+        * assert (cmp := eq'). rewrite <- eq in eq'.  clear eq inf sup. rewrite <- H5, <-H7 in cmp.
+            destruct x,x0. inversion H4. inversion H6.  simpl in cmp. subst. constructor. constructor... 
+
+        (* z1 > z2 *)
+        * apply Z.lt_gt in sup'. assert (cmp := sup'). apply <- sup in sup'.  clear inf eq sup.
+          destruct x, x0. inversion H4. inversion H6. constructor. apply S_IfFalse.
+            + econstructor... subst. simpl in *. unfold Z.ltb. now rewrite cmp.
+            + apply S_IfTrue with one ; subst... split... subst.  eapply C_E_BinOpTrue... 
+                    rewrite Z.gtb_ltb. rewrite Z.ltb_lt. now rewrite <- Z.gt_lt_iff.
+Admitted.
+
+
+
+
+Lemma semantics_of_the_binop_macro_int :
+    forall (Ω:Ω) (M:𝓜) (op:fsl_binop_int) c r e1 e2 v1 v2 z1 z2 (ir: Int.inRange (⋄ (□ op) z1 z2) ) l1 l2 lr,
+    type_of_value ((fst Ω) c) = Some C_Int ->
+    Ω ⋅ M |= e1 ⇝ z1 ->
+    Ω ⋅ M |= e2 ⇝ z2 ->
+    let zr := ⋄ (□ op) z1 z2 in
+
+    (fst Ω) v1 = Some (VMpz l1) /\  (fst Ω) v2 = Some (VMpz l2) /\ ( (fst Ω) r = Some (VMpz lr) ) ->
+    exists M', forall v n, (fst Ω) v = Some (VMpz n) ->
+    ~ ((fst Ω) v1 = (fst Ω) v) /\ ~ ((fst Ω) v2 = (fst Ω) v)  -> M n = M' n -> 
+    Ω ⋅ M |= (binop_ASSGN op (C_Int,c) e1 e2 r v1 v2) => ((fst Ω){c\zr ⁱⁿᵗ ir}, snd Ω) ⋅ M'
+    .
+
+Proof with eauto with rac_hint.
+    intros. destruct H2 as (v1l & v2l & rl).  
+    assert (NotInt : 
+    exists M', forall v n, (fst Ω) v = Some (VMpz n) ->
+    ~ ((fst Ω) v1 = (fst Ω) v) /\ ~ ((fst Ω) v2 = (fst Ω) v)  -> M n = M' n -> 
+    Ω ⋅ M |= <{
+
+        (mpz_ASSGN v1 e1);
+        (mpz_ASSGN v2 e2);
+        (Definitions.op op r v1 v2);
+        (int_ASSGN c (C_Id r Mpz))
+        
+        }> => ((fst Ω){c\zr ⁱⁿᵗ ir}, snd Ω) ⋅ M'
+    
+    ). {
+        exists M{lr\zr,l2\z2,l1\z1}. intros. 
+    apply GMP_Seq with Ω M{l1\z1}. apply semantics_of_the_mpz_assgn_macro...
+    apply GMP_Seq with Ω M{l2\z2,l1\z1}. apply semantics_of_the_mpz_assgn_macro... admit.
+    apply GMP_Seq with Ω M{lr\zr,l2\z2,l1\z1}. 
+    apply S_op with l1 l2...
+    * constructor. admit.
+    * unfold p_map. simpl. destruct Nat.eq_dec.
+        + admit.
+        + now destruct Nat.eq_dec.
+    * constructor. admit.
+    * unfold p_map. simpl. now destruct Nat.eq_dec.
+    * apply semantics_of_the_int_assgn_macro...  apply M_Mpz with lr.
+        +  constructor. admit. 
+        +  unfold p_map. simpl. now destruct Nat.eq_dec. 
+    }
+    
+    unfold binop_ASSGN. destruct (ty e1) eqn:T1, (ty e2) eqn:T2 ; 
+    (* get rid of impossible void type *)
+    try (unfold ty in T2 ; destruct e2 eqn:X; try easy ; subst ; inversion H1 ; inversion H5; easy) ;
+    try (unfold ty in T1;  destruct e1 eqn:X; try easy; subst; inversion H0; inversion H5; easy);
+    (* when ty e1 & ty e2 != int *)
+    try (exists M{lr\zr,l2\z2,l1\z1} ; intros ; now apply NotInt). clear NotInt.
+
+
+    exists M. intros. inversion H0 ; inversion H1;  subst ; constructor ; constructor ; admit.
+Admitted.
+
+
+
+Lemma semantics_of_the_binop_macro_mpz :
+    forall (Ω:Ω) (M:𝓜) (op:fsl_binop_int) c y r e1 e2 v1 v2 z1 z2 l1 l2,
+    type_of_value ((fst Ω) c) = Some C_Int ->
+    Ω ⋅ M |= e1 ⇝ z1 ->
+    Ω ⋅ M |= e2 ⇝ z2 ->
+   
+    let zr := ⋄ (□ op) z1 z2 in
+    (fst Ω) v1 = Some (VMpz l1) /\  (fst Ω) v2 = Some (VMpz l2) /\  (fst Ω) c = Some (VMpz y) ->
+    exists M', forall v n, (fst Ω) v = Some (VMpz n) ->
+    ~ ((fst Ω) v1 = (fst Ω) v) /\ ~ ((fst Ω) v2 = (fst Ω) v)  -> M n = M' n -> 
+    Ω ⋅ M |= (binop_ASSGN op (T_Ext Mpz,c) e1 e2 r v1 v2) => Ω ⋅ M'{y\zr}
+    .
+Proof with eauto with rac_hint.
+    intros. exists M{l2\z2,l1\z1}. intros. destruct H2 as (v1l & v2l & rl). unfold binop_ASSGN.
+    apply GMP_Seq with Ω M{l1\z1}.
+    - apply semantics_of_the_mpz_assgn_macro...
+    - apply GMP_Seq with Ω M{l2\z2,l1\z1}. 
+        * apply semantics_of_the_mpz_assgn_macro... admit.
+        * apply S_op with l1 l2  ...
+            + constructor. admit. 
+            + unfold p_map. simpl. destruct Nat.eq_dec.
+                ++ admit.
+                ++ now destruct Nat.eq_dec.
+            + constructor. admit.
+            + unfold p_map. simpl. now destruct Nat.eq_dec.
+Admitted.
+
+
+(* Preservation of the semantics *)
+
+Open Scope mini_fsl_scope.
+
+Lemma semantics_of_term_translation : 
+    forall (t:fsl_term) Ω Γ Ψ, 
+    I1 Ω Γ ->
+    I2 Ψ ->
+    (exists (z:ℤ), Ω |= t => z)
+        <-> True.
+Proof.
+Admitted.
